Add lemmas for reduction consistent proof theory. Ready to prove classical propositional logic is stronger than intuitionistic.

PropositionalLogic/KripkeSemantics.v
@@ -1,78 +1,84 @@
 Require Import Logic.LogicBase.
 Require Import Logic.SyntacticReduction.
-Require Import Logic.KripkeModel.
 Require Import Logic.PropositionalLogic.Syntax.
 Require Import Coq.Logic.Classical_Prop.
 Require Import Coq.Classes.RelationClasses.
 
 Local Open Scope logic_base.
 Local Open Scope PropositionalLogic.
-(*
-Class KripkeIntuitionisticSemantics (L: Language) {nL: NormalLanguage L} {pL: PropositionalLanguage L} (SM: Semantics L) {rcSM: ReductionConsistentSemantics IntuitionisticReduction SM}: Type := {
-  Kripke_model: Type;
-  frame_worlds: Kripke_model -> Type;
-  frame_relation: forall {m: Kripe_model}, frame_type m -> frame_type m -> Prop;
-  build_model: forall m: Kripke_model, frame_type m -> model;
-  sem_impp: forall m x y, m |= x --> y <-> (m |= x -> m |= y);
-  sem_negp: forall m x, m |= ~~ x <-> ~ m |= x;
-  sem_truep: forall m, m |= TT
+
+Class PreKripkeSemantics (L: Language) (SM: Semantics L): Type := {
+  Kmodel: Type;
+  Kworlds: Kmodel -> Type;
+  build_model: forall M: Kmodel, Kworlds M -> model
 }.
-*)
+
+Notation "'KRIPKE:'  M , m" := (build_model M m) (at level 59, no associativity) : logic_base.
+
+Class KripkeIntuitionisticSemantics (L: Language) {nL: NormalLanguage L} {pL: PropositionalLanguage L} (SM: Semantics L) {rcSM: ReductionConsistentSemantics IntuitionisticReduction SM} {pkSM: PreKripkeSemantics L SM}: Type := {
+  Korder: forall {M: Kmodel}, Kworlds M -> Kworlds M -> Prop; (* <= *)
+  sat_mono: forall M m n x, Korder m n -> KRIPKE: M , n |= x -> KRIPKE: M , m |= x;
+  sat_impp: forall M m x y, KRIPKE: M , m |= x --> y <-> (forall n, Korder n m -> KRIPKE: M , n |= x -> KRIPKE: M , n |= y);
+  sat_andp: forall M m x y, KRIPKE: M , m |= x && y <-> (KRIPKE: M , m |= x /\ KRIPKE: M , m |= y);
+  sat_orp: forall M m x y, KRIPKE: M , m |= x || y <-> (KRIPKE: M , m |= x \/ KRIPKE: M , m |= y);
+  sat_falsep: forall M m, ~ KRIPKE: M , m |= FF
+}.
+
 Module KripkeSemantics.
 
 Import PropositionalLanguage.
 
 Record frame: Type := {
-  frame_type: Type;
-  frame_order: relation frame_type; (* <= *)
-  frame_preorder: PreOrder frame_order
+  underlying_set:> Type;
+  Korder: relation underlying_set; (* <= *)
+  Korder_preorder: PreOrder Korder
 }.
 
-Infix "<=" := (frame_order _): KripkeSemantics.
+Infix "<=" := (Korder _): KripkeSemantics.
 
 Local Open Scope KripkeSemantics.
 
-Definition sem (f: frame) := sig (fun s: Ensemble (frame_type f) => forall x y, x <= y -> s y -> s x).
+Definition sem (f: frame) := sig (fun s: Ensemble f => forall x y, x <= y -> s y -> s x).
 
-Program Definition sem_and {f: frame} (X: sem f) (Y: sem f): sem f :=
-  fun x: frame_type f => X x /\ Y x.
+Program Definition sem_and {F: frame} (X: sem F) (Y: sem F): sem F :=
+  fun x: F => X x /\ Y x.
 Next Obligation.
   split.
   + eapply (proj2_sig X); eauto.
   + eapply (proj2_sig Y); eauto.
 Qed.
 
-Program Definition sem_or {f: frame} (X: sem f) (Y: sem f): sem f :=
-  fun x: frame_type f => X x \/ Y x.
+Program Definition sem_or {F: frame} (X: sem F) (Y: sem F): sem F :=
+  fun x: F => X x \/ Y x.
 Next Obligation.
   destruct H0; [left | right].
   + eapply (proj2_sig X); eauto.
   + eapply (proj2_sig Y); eauto.
 Qed.
 
-Program Definition sem_imp {f: frame} (X: sem f) (Y: sem f): sem f :=
-  fun x: frame_type f =>
-    forall y: frame_type f, y <= x -> X y -> Y y.
+Program Definition sem_imp {F: frame} (X: sem F) (Y: sem F): sem F :=
+  fun x: F =>
+    forall y: F, y <= x -> X y -> Y y.
 Next Obligation.
   revert H2; apply H0.
-  pose proof @PreOrder_Transitive _ _ (frame_preorder f).
+  pose proof @PreOrder_Transitive _ _ (Korder_preorder F).
   transitivity x; auto.
 Qed.
 
-Program Definition sem_true {f: frame}: sem f :=
-  fun x: frame_type f => True.
+Program Definition sem_true {F: frame}: sem F :=
+  fun x: F => True.
 
-Program Definition sem_false {f: frame}: sem f :=
-  fun x: frame_type f => False.
+Program Definition sem_false {F: frame}: sem F :=
+  fun x: F => False.
 
-Definition sem_neg {f: frame} (X: sem f): sem f :=
+Definition sem_neg {F: frame} (X: sem F): sem F :=
   sem_imp X sem_false.
 
-Definition sem_iff {f: frame} (X: sem f) (Y: sem f): sem f :=
+Definition sem_iff {F: frame} (X: sem F) (Y: sem F): sem F :=
   sem_and (sem_imp X Y) (sem_imp Y X).
 
-Definition denotation {Var: Type} (f: frame) (eval: Var -> sem f): expr Var -> sem f :=
-  fix denotation (x: expr Var): sem f:=
+Definition denotation {Var: Type} (F: frame) (eval: Var -> sem F): expr Var -> sem F :=
+  fix denotation (x: expr Var): sem F:=
   match x with
   | andp y z => sem_and (denotation y) (denotation z)
   | orp y z => sem_or (denotation y) (denotation z)
@@ -83,20 +89,6 @@ Definition denotation {Var: Type} (f: frame) (eval: Var -> sem f): expr Var -> s
   | falsep => sem_false
   | varp p => eval p
   end.
-
-Record model {Var: Type} : Type := {
-  model_frame: frame;
-  model_var: Var -> sem model_frame;
-  elm: frame_type model_frame
-}.
-
-Implicit Arguments model.
-
-Instance SM (Var: Type): Semantics (PropositionalLanguage.L Var) :=
-  Build_Semantics (PropositionalLanguage.L Var) (model Var) (fun m x => proj1_sig (denotation (model_frame m) (model_var m) x) (elm m)).
-
-Local Open Scope logic_base.
-Local Open Scope PropositionalLogic.
 
 Lemma ImpAndOrAsPrime_consistent {Var: Type}:
   forall x y: expr Var,
@@ -124,43 +116,78 @@ Proof.
   + hnf; auto.
 Qed.
 
-Lemma RPC {Var: Type}: ReductionPropagationConsistent (SM Var).
+Lemma RPC_aux {Var: Type}: forall  F eval (x y: expr Var) sp,
+  (forall v, proj1_sig (denotation F eval x) v <-> proj1_sig (denotation F eval y) v) ->
+  (forall v, proj1_sig (denotation F eval (single_propagation_denote sp x)) v <->
+             proj1_sig (denotation F eval (single_propagation_denote sp y)) v).
+Proof.
+  intros.
+  destruct sp; intros.
+  + specialize (H v).
+    simpl in *.
+    tauto.
+  + specialize (H v).
+    simpl in *.
+    tauto.
+  + specialize (H v).
+    simpl in *.
+    tauto.
+  + specialize (H v).
+    simpl in *.
+    tauto.
+  + simpl in *.
+    split; intros HH u Hu; specialize (HH u Hu); specialize (H u); tauto.
+  + simpl in *.
+    split; intros HH u Hu; specialize (HH u Hu); specialize (H u); tauto.
+  + simpl in *.
+    apply Morphisms_Prop.and_iff_morphism.
+    - simpl in *.
+      split; intros HH u Hu; specialize (HH u Hu); specialize (H u); tauto.
+    - simpl in *.
+      split; intros HH u Hu; specialize (HH u Hu); specialize (H u); tauto.
+  + simpl in *.
+    apply Morphisms_Prop.and_iff_morphism.
+    - simpl in *.
+      split; intros HH u Hu; specialize (HH u Hu); specialize (H u); tauto.
+    - simpl in *.
+      split; intros HH u Hu; specialize (HH u Hu); specialize (H u); tauto.
+  + simpl in *.
+    split; intros HH u Hu; specialize (HH u Hu); specialize (H u); tauto.
+Qed.
+
+End KripkeSemantics.
+
+Module KripkeSemantics_All.
+
+Import KripkeSemantics.
+
+Record Kmodel {Var: Type} : Type := {
+  underlying_frame :> frame;
+  Kvar: Var -> sem underlying_frame
+}.
+
+Record model {Var: Type}: Type := {
+  underlying_model :> @Kmodel Var;
+  elm: underlying_model
+}.
+
+Implicit Arguments model.
+
+Instance SM (Var: Type): Semantics (PropositionalLanguage.L Var) :=
+  Build_Semantics (PropositionalLanguage.L Var)
+   (@model Var)
+   (fun M x => proj1_sig (denotation M (Kvar M) x) (elm M)).
+
+Local Open Scope logic_base.
+Local Open Scope PropositionalLogic.
+
+Lemma RPC {Var: Type}: ReductionPropagationConsistentSemantics (SM Var).
 Proof.
   hnf; intros; simpl in *.
-  destruct m as [F eval v].
-  pose proof (fun v => H (Build_model _ F eval v)).
-  revert v; simpl in H0; clear H.
-  destruct sp; intros.
-  + specialize (H0 v).
-    simpl in *.
-    tauto.
-  + specialize (H0 v).
-    simpl in *.
-    tauto.
-  + specialize (H0 v).
-    simpl in *.
-    tauto.
-  + specialize (H0 v).
-    simpl in *.
-    tauto.
-  + simpl in *.
-    split; intros HH u Hu; specialize (HH u Hu); specialize (H0 u); tauto.
-  + simpl in *.
-    split; intros HH u Hu; specialize (HH u Hu); specialize (H0 u); tauto.
-  + simpl in *.
-    apply Morphisms_Prop.and_iff_morphism.
-    - simpl in *.
-      split; intros HH u Hu; specialize (HH u Hu); specialize (H0 u); tauto.
-    - simpl in *.
-      split; intros HH u Hu; specialize (HH u Hu); specialize (H0 u); tauto.
-  + simpl in *.
-    apply Morphisms_Prop.and_iff_morphism.
-    - simpl in *.
-      split; intros HH u Hu; specialize (HH u Hu); specialize (H0 u); tauto.
-    - simpl in *.
-      split; intros HH u Hu; specialize (HH u Hu); specialize (H0 u); tauto.
-  + simpl in *.
-    split; intros HH u Hu; specialize (HH u Hu); specialize (H0 u); tauto.
+  destruct m as [M v].
+  pose proof (fun v => H (Build_model _ M v)).
+  revert v; simpl in H0; clear H. simpl.
+  apply RPC_aux; auto.
 Qed.
 
 Instance rcSM (Var: Type): ReductionConsistentSemantics IntuitionisticReduction (SM Var).
@@ -168,12 +195,96 @@ Proof.
   apply Build_ReductionConsistentSemantics.
   + hnf; intros.
     revert x y H m.
-    repeat apply disjunction_reduce_consistent; intros.
+    repeat apply disjunction_reduce_consistent_semantics; intros.
     - apply ImpAndOrAsPrime_consistent; auto.
     - apply ReduceIff_consistent; auto.
     - apply ReduceTrue_consistent; auto.
   + apply RPC.
 Qed.
 
-End KripkeSemantics.
+Instance pkSM (Var: Type): PreKripkeSemantics (PropositionalLanguage.L Var) (SM Var) :=
+  Build_PreKripkeSemantics _ (SM Var)
+   Kmodel
+   (fun M => M)
+   (fun M m => Build_model _ M m).
+
+Instance kiSM (Var: Type): KripkeIntuitionisticSemantics (PropositionalLanguage.L Var) (SM Var).
+Proof.
+  apply (Build_KripkeIntuitionisticSemantics _ _ _ _ _ (pkSM Var) (fun M => Korder M)).
+  + hnf; simpl; intros.
+    eapply (proj2_sig (denotation M (Kvar M) x)); eauto.
+  + split; auto.
+  + split; auto.
+  + split; auto.
+  + intros; simpl. auto.
+Qed.
+
+End KripkeSemantics_All.
+
+Module KripkeSemantics_Reflexive.
+
+Import KripkeSemantics.
+
+Import KripkeSemantics.
+
+Record Kmodel {Var: Type} : Type := {
+  underlying_frame :> frame;
+  Kvar: Var -> sem underlying_frame;
+  frame_reflexive: Reflexive (Korder underlying_frame)
+}.
+
+Record model {Var: Type}: Type := {
+  underlying_model :> @Kmodel Var;
+  elm: underlying_model
+}.
+
+Implicit Arguments model.
+
+Instance SM (Var: Type): Semantics (PropositionalLanguage.L Var) :=
+  Build_Semantics (PropositionalLanguage.L Var)
+   (@model Var)
+   (fun M x => proj1_sig (denotation M (Kvar M) x) (elm M)).
+
+Local Open Scope logic_base.
+Local Open Scope PropositionalLogic.
+
+Lemma RPC {Var: Type}: ReductionPropagationConsistentSemantics (SM Var).
+Proof.
+  hnf; intros; simpl in *.
+  destruct m as [M v].
+  pose proof (fun v => H (Build_model _ M v)).
+  revert v; simpl in H0; clear H. simpl.
+  apply RPC_aux; auto.
+Qed.
+
+Instance rcSM (Var: Type): ReductionConsistentSemantics IntuitionisticReduction (SM Var).
+Proof.
+  apply Build_ReductionConsistentSemantics.
+  + hnf; intros.
+    revert x y H m.
+    repeat apply disjunction_reduce_consistent_semantics; intros.
+    - apply ImpAndOrAsPrime_consistent; auto.
+    - apply ReduceIff_consistent; auto.
+    - apply ReduceTrue_consistent; auto.
+  + apply RPC.
+Qed.
+
+Instance pkSM (Var: Type): PreKripkeSemantics (PropositionalLanguage.L Var) (SM Var) :=
+  Build_PreKripkeSemantics _ (SM Var)
+   Kmodel
+   (fun M => M)
+   (fun M m => Build_model _ M m).
+
+Instance kiSM (Var: Type): KripkeIntuitionisticSemantics (PropositionalLanguage.L Var) (SM Var).
+Proof.
+  apply (Build_KripkeIntuitionisticSemantics _ _ _ _ _ (pkSM Var) (fun M => Korder M)).
+  + hnf; simpl; intros.
+    eapply (proj2_sig (denotation M (Kvar M) x)); eauto.
+  + split; auto.
+  + split; auto.
+  + split; auto.
+  + intros; simpl. auto.
+Qed.
+
+End KripkeSemantics_Reflexive.
 
