PropositionalLogic/Classical2Intuitionistic.v
@@ -1,0 +1,26 @@
+Require Import Logic.LogicBase.
+Require Import Logic.SyntacticReduction.
+Require Import Logic.PropositionalLogic.Syntax.
+Require Import Logic.PropositionalLogic.MinimunPropositionalLogic.
+Require Import Logic.PropositionalLogic.ClassicalPropositionalLogic.
+Require Import Logic.PropositionalLogic.IntuitionisticPropositionalLogic.
+
+Local Open Scope logic_base.
+Local Open Scope PropositionalLogic.
+
+Definition ClassicalImpAndOrAsPrimeReduction {L: Language} {nL: NormalLanguage L} {pL: PropositionalLanguage L} {Gamma: ProofTheory L} {nGamma: NormalProofTheory L Gamma} {mpGamma: MinimunPropositionalLogic L Gamma} {rcGamma: ReductionConsistentProofTheory MendelsonReduction Gamma} {cpGamma: ClassicalPropositionalLogic L Gamma}:
+  AtomicReductionConsistentProvable ImpAndOrAsPrime.atomic_reduce Gamma.
+Proof.
+  hnf; intros.
+  destruct H.
+  +
+Abort.
+
+Definition ClassicalIntuitionisticReduction {L: Language} {nL: NormalLanguage L} {pL: PropositionalLanguage L} {Gamma: ProofTheory L} {nGamma: NormalProofTheory L Gamma} {mpGamma: MinimunPropositionalLogic L Gamma} {rcGamma: ReductionConsistentProofTheory MendelsonReduction Gamma} {cpGamma: ClassicalPropositionalLogic L Gamma}:
+  ReductionConsistentProofTheory IntuitionisticReduction Gamma.
+Proof.
+  apply Build2_ReductionConsistentProofTheory.
+  + simpl.
+    repeat apply disjunction_reduce_consistent_provable.
+Abort.
+
